well-formedness

theories/sim/refl.v
@@ -3,7 +3,42 @@ From stbor.sim Require Import refl_step.
 
 Set Default Proof Using "Type".
 
+(** Enable use of [Forall] in recursion. *)
+Lemma Forall_id {A: Type} (P: A → Prop) (l: list A) :
+  Forall P l ↔ Forall id (map P l).
+Proof.
+  induction l; simpl; first by eauto using Forall_nil.
+  split; intros [??]%Forall_cons_1; apply Forall_cons; simpl; tauto.
+Qed.
+
+(** "Well-formed" code doen't contain literal
+pointers, places or administrative operations (init_call/end_call).
+Defined by recursion to make sure we don't miss a case. *)
+Fixpoint scalar_wf (a: scalar) : Prop :=
+  match a with
+  | ScPoison | ScInt _ | ScFnPtr _ => True
+  | ScnPtr => False
+  end.
+Definition value_wf (v: value) : Prop := Forall scalar_wf v.
+Fixpoint expr_wf (e: expr) : Prop :=
+  match e with
+  (* Structural cases. *)
+  | Val v => value_wf v
+  | Call f args => expr_wf f ∧ Forall id (map expr_wf args)
+  | Case e branches => expr_wf e ∧ Forall id (map expr_wf branches)
+  | Var _ | Alloc _ => True
+  | Deref e _ | Ref e  | Copy e | Retag e _ =>
+    expr_wf e
+  | Proj e1 e2 | Conc e1 e2 | BinOp _ e1 e2 | Let _ e1 e2 | Write e1 e2 =>
+    expr_wf e1 ∧ expr_wf e2
+  (* Forbidden cases. *)
+  | InitCall e | EndCall e => False
+  | Place _ _ _ => False
+  | Free _ => False (* TODO: We'd like to support deallocation! *)
+  end.
+
 Theorem sim_mod_fun_refl f :
+  expr_wf f.(fun_body) →
   ⊨ᶠ f ≥ f.
 Proof.
 Admitted.
@@ -15,4 +50,4 @@ Proof.
   { intros ??. rewrite lookup_empty. done. }
   apply sim_mod_funs_insert; try done.
   apply sim_mod_fun_refl.
-Qed.
+Admitted.
