theories/opt/ex3.v
@@ -32,13 +32,6 @@ Definition ex3_opt_2 : function :=
     Call #[ScFnPtr "f"] []
   .
 
-Lemma ex3_sim_fun fs ft : ⊨ᶠ{fs,ft} ex3 ≥ ex3_opt_1.
+Lemma ex3_sim_fun : ⊨ᶠ ex3 ≥ ex3_opt_1.
 Proof.
-  intros r es et vls vlt σs σt FREL SUBSTs SUBSTt.
-  destruct vls as [|vs []]; [done| |done].  simpl in SUBSTs.
-  destruct vlt as [|vt []]; [done| |done].  simpl in SUBSTt. simplify_eq.
-
-  (* InitCall *)
-  exists 10%nat.
-  apply sim_body_init_call. simpl.
 Abort.
